Finish the DRF-PF

src/lang/Language.v
@@ -8,6 +8,26 @@ Require Import Time.
 Set Implicit Arguments.
 
 Module Language.
+  Inductive receptive
+            (state:Type)
+            (step: forall (e:ProgramEvent.t) (s1:state) (s2:state), Prop): Prop :=
+  | receptive_intro
+      (READ:
+         forall st loc ord
+           val1 st1
+           val2
+           (STEP1: step (ProgramEvent.read loc val1 ord) st st1),
+         exists st2,
+           <<STEP2: step (ProgramEvent.read loc val2 ord) st st2>>)
+      (UPDATE:
+         forall st loc or ow
+           vr1 vw1 st1
+           vr2
+           (STEP1: step (ProgramEvent.update loc vr1 vw1 or ow) st st1),
+         exists vw2 st2,
+           <<STEP2: step (ProgramEvent.update loc vr2 vw2 or ow) st st2>>)
+  .
+
   Structure t := mk {
     syntax: Type;
     state: Type;
@@ -15,5 +35,7 @@ Module Language.
     init: syntax -> state;
     is_terminal: state -> Prop;
     step: forall (e:ProgramEvent.t) (s1:state) (s2:state), Prop;
+
+    RECEPTIVE: receptive step;
   }.
 End Language.
